@prefix owl: <http://www.w3.org/2002/07/owl#> .
@prefix rdfs: <http://www.w3.org/2000/01/rdf-schema#> .
@prefix ewe: <http://gsi.dit.upm.es/ontologies/ewe/ns/> .
@prefix ewe: <http://gsi.dit.upm.es/ontologies/emo/ns/> .
@prefix oaa: <http://gsi.dit.upm.es/ontologies/oaa/ns/> .
@prefix onyx: <http://gsi.dit.upm.es/ontologies/onyx/ns/> .

###################################
# Channel definition
###################################

emo:ContextSensor a owl:Class ;    
    rdfs:label "Context Sensor" ;
    rdfs:comment "This channel represents a context sensor able to detect emotions and activites." ;
    rdfs:subClassOf ewe:Channel .

###################################
# Events definition
###################################

emo:EmotionDetected a owl:Class ;
    rdfs:label "Emotion Detected" ;
    rdfs:comment "This Trigger fires every time your context sensor detects an emotion." ;
    ewe:hasInputParameter emo:Emotion ;
    rdfs:subclassOf ewe:Event ;
    rdfs:domain emo:ContextSensor .

emo:ActivityDetected a owl:Class ;
    rdfs:label "Activity Detected" ;
    rdfs:comment "This Trigger fires every time your context sensor detects an activity." ;
    ewe:hasInputParameter emo:Activity ;
    rdfs:subclassOf ewe:Event ;
    rdfs:domain emo:ContextSensor .

###################################
# Parameters definition
###################################

emo:Emotion a owl:Class ;
	rdfs:label "Emotion" ;
	rdfs:subclassOf ewe:InputParameter ;
	rdfs:subclassOf onyx:Emotion ;
	rdfs:domain emo:ContextSensor .

emo:Activity a owl:Class ;
	rdfs:label "Activity" ;
	rdfs:subclassOf ewe:InputParameter ;
	rdfs:subclassOf oaa:Activity ;
	rdfs:domain emo:ContextSensor .